

# Mathematical foundations for Machine learning

Name: B. Haripriya

ID : 2025AA05640

## Question

Shop Number	Operating Hours (x)	Consumption (y)
1	1	3
2	2	5
3	4	9
4	6	13
5	8	17

(a)  $\hat{y}_i = w_0 + w_1 x_i$

$$J(w_0, w_1) = \frac{1}{2} \sum_{i=1}^5 (\hat{y}_i - y_i)^2$$

$$(a \pm b)^2 = a^2 \pm 2ab + b^2$$

$$\Rightarrow (a+b-c)^2 = (a+b)^2 - 2(a+b)c + c^2$$

$$\Rightarrow J(w_0, w_1) = \frac{1}{2} \sum_{i=1}^5 (\hat{y}_i - y_i)^2$$

$$= \frac{1}{2} \sum_{i=1}^5 (w_0 + w_1 x_i - y_i)^2 \quad \hookrightarrow \textcircled{1}$$

$$\Rightarrow \text{Now, } (w_0 + w_1 x_i - y_i)^2 = (w_0 + w_1 x_i)^2 - 2(w_0 + w_1 x_i)y_i + y_i^2 \quad \hookrightarrow \textcircled{2}$$

$\Rightarrow$  From  $\textcircled{1}$  &  $\textcircled{2}$

$$J(w_0, w_1) = \frac{1}{2} \sum_{i=1}^5 \left( \underbrace{w_0^2}_a + \underbrace{2w_0 w_1 x_i}_b + \underbrace{w_1^2 x_i^2}_c - \underbrace{2w_0 y_i}_d - \underbrace{2w_1 x_i y_i}_e + \underbrace{y_i^2}_f \right) \quad \hookrightarrow \textcircled{3}$$

$$\Rightarrow a = \sum_{i=1}^5 w_0^2 = 5w_0^2$$



$$\begin{aligned}
 b &= \sum_{i=1}^5 2\omega_0 \omega_1 x_i = 2\omega_0 \omega_1 \sum_{i=1}^5 x_i \\
 &= 2\omega_0 \omega_1 (1+2+4+6+8) \\
 &= 42\omega_0 \omega_1
 \end{aligned}$$

$$\begin{aligned}
 c &= \sum_{i=1}^5 \omega_1^2 x_i^2 = \omega_1^2 \sum_{i=1}^5 x_i^2 \\
 &= \omega_1^2 (1^2 + 2^2 + 4^2 + 6^2 + 8^2) = 121\omega_1^2
 \end{aligned}$$

$$\begin{aligned}
 d &= -2\omega_0 \sum_{i=1}^5 y_i = -2\omega_0 (3+5+9+13+17) \\
 &= -94\omega_0
 \end{aligned}$$

$$\begin{aligned}
 e &= -2\omega_1 \sum_{i=1}^5 x_i y_i = -2\omega_1 (1 \times 3 + 2 \times 5 + 4 \times 9 \\
 &\quad + 6 \times 13 + 8 \times 17) = -526\omega_1
 \end{aligned}$$

$$\begin{aligned}
 f &= \sum_{i=1}^5 y_i^2 = (3^2 + 5^2 + 9^2 + 13^2 + 17^2) \\
 &= 573
 \end{aligned}$$

from (3) :-

$$J(\omega_0, \omega_1) = \frac{1}{2} (5\omega_0^2 + 42\omega_0\omega_1 + 121\omega_1^2 - 94\omega_0 - 526\omega_1 + 573)$$

$$J(\omega_0, \omega_1) = 2.5\omega_0^2 + 21\omega_0\omega_1 + 60.5\omega_1^2 - 47\omega_0 - 263\omega_1 + 286.5 \rightarrow (4)$$

$$\frac{\partial J}{\partial \omega_0} = 5\omega_0 + 21\omega_1 - 47 \rightarrow (5)$$

$$\frac{\partial J}{\partial \omega_1} = 21\omega_0 + 121\omega_1 - 263 \rightarrow (6)$$

$$\frac{\partial^2 J}{\partial \omega_0^2} = 5 ; \frac{\partial^2 J}{\partial \omega_1^2} = 121, \frac{\partial^2 J}{\partial \omega_0 \partial \omega_1} = 21,$$

$$\frac{\partial^2 J}{\partial \omega_1 \partial \omega_0} = 21$$



$$a) H = \begin{bmatrix} \frac{2^2 J}{2\omega_0^2} & \frac{2^2 J}{2\omega_0 \omega_1} \\ \frac{2^2 J}{2\omega_1 \omega_0} & \frac{2^2 J}{2\omega_1^2} \end{bmatrix}$$

$$= \begin{bmatrix} 5 & 21 \\ 21 & 121 \end{bmatrix}$$

First leading principal minor  $= 5 > 0$

$$\det(H) = 5 \times 121 - (21) \times (21)$$

$$= \underline{146}$$

$$= 164 > 0$$

$\therefore H$  is +ve definite

$\Rightarrow$  A strictly convex function requires  $H$  to be +ve definite

$\Rightarrow \therefore J(\omega_0, \omega_1)$  is strictly convex.

$$(b) \nabla J = \begin{bmatrix} \frac{\partial J}{\partial w_0} \\ \frac{\partial J}{\partial w_1} \end{bmatrix} = \begin{bmatrix} 5w_0 + 21w_1 - 47 \\ 21w_0 + 121w_1 - 263 \end{bmatrix}$$

(from 5 & 6)  $\rightarrow$  ⑦

(c) (i.) Constant learning rate =  $\eta$   
 $= 0.05$

$$(0) \quad w_0 = 2, \quad w_1 = 2$$

from ⑦

$$\nabla J = \begin{bmatrix} 5 \times 2 + 21 \times 2 - 47 \\ 21 \times 2 + 121 \times 2 - 263 \end{bmatrix} = \begin{bmatrix} 5 \\ 21 \end{bmatrix}$$

$\rightarrow$  ⑧



(i)  $t=1$ , Iteration 1

$$w_0^{(0)} - \eta \frac{\partial J}{\partial w_0} = 2 - 0.05 \times 5 = \underline{1.75}$$

$$w_1^{(1)} = w_1^{(0)} - \eta \frac{\partial J}{\partial w_1} = 2 - 0.05(21) \\ = \underline{0.95}$$

After iteration 1:-

$$w_0^{(1)} = 1.75, \quad w_1^{(1)} = 0.95$$

(ii)  $t=2$  Iteration 2:-

$$\frac{\partial J}{\partial w_0} = 5w_0 + 21w_1 - 47 \\ = 5(1.75) + 21(0.95) - 47 \\ = \underline{-18.3}$$

$$\frac{\partial J}{\partial w_1} = 21w_0 + 121w_1 - 263 \\ = 21(1.75) + 121(0.95) - 263 \\ = \underline{-111.3}$$

$$\therefore \nabla J = \begin{bmatrix} -18.3 \\ -111.3 \end{bmatrix}$$

$$w_0^{(2)} = w_0^{(1)} - \frac{\eta \nabla J}{\partial w_0}$$

$$w_1^{(2)} = w_1^{(1)} - \eta \frac{\nabla J}{\partial w_1}$$

$$w_0^{(2)} = 1.75 - 0.05 (-18.3) = \boxed{2.665} \quad (c)$$

$$w_1^{(2)} = 0.95 - 0.05 (-111.3) = \boxed{6.515}$$

⇒ After Iteration 2,

$$w_0^{(2)} = 2.665 \quad \& \quad w_1^{(2)} = 6.515$$

2.  $\eta_t = \eta_0 e^{-kt}$ ,  $\eta_0 = 0.1$ ,  $k = 0.4$ ,  
 $t = 1, 2, 3, \dots$



$$w_0^{(0)} = 2, \quad w_1^{(0)} = 2$$

(i) Iteration 1 :-

$$t=1 :-$$

$$\eta_1 = \eta_0 e^{-0.4 \times 1} = 0.067$$

$$\nabla J = \begin{bmatrix} 5 \\ 21 \end{bmatrix} \quad [\text{from (3)}]$$

(c) 2. (i)  $w_0^{(1)} = w_0^{(0)} - \eta_1 \frac{\partial J}{\partial w_0}$

$$= 2 - 0.067 \times 5$$

$$= 1.665$$

$$w_1^{(1)} = w_1^{(0)} - \eta_1 \frac{\partial J}{\partial w_1}$$

$$= 2 - 0.067 \times 21$$

$$= 0.593$$

$$\therefore w_0^{(1)} = 1.665, \quad w_1^{(1)} = 0.593 \quad \text{after iteration 1}$$

(ii) Iteration 2,  $t=2$  :-

$$n_2 = n_0 e^{-0.4 \times 2} = 0.1 e^{-0.8}$$

$$\boxed{n_2 = 0.0449}$$

$$\begin{aligned} \Rightarrow \frac{2J}{2w_0} &= 5w_0 + 21w_1 - 47 \\ &= 5(1.665) + 21(0.593) - 47 \\ &= \underline{-26.222} \end{aligned}$$

$$\begin{aligned} \Rightarrow \frac{2J}{2w_1} &= 21w_0 + 121w_1 - 263 \\ &= 21(1.665) + 121(0.593) - 263 \\ &= \underline{-156.282} \end{aligned}$$

$$\begin{aligned} \Rightarrow w_0^{(2)} &= w_0^{(1)} - \eta \frac{2J}{2w_0} \\ &= 1.665 - 0.0449(-26.222) \\ &= \underline{2.8424} \end{aligned}$$



$$\Rightarrow \omega_1^{(2)} = \omega_1^{(1)} - \eta_2 \frac{2J}{2\omega_1}$$

$$= 0.593 - 0.0449 (-156.282)$$

$$= \underline{7.6101}$$

$$\therefore \text{Iteration 2, } \omega_0^{(2)} = 2.8424$$

$$\& \omega_1^{(2)} = \underline{7.6101}$$

(c)  $\omega_0^{(1)} = 1.75, \omega_1^{(1)} = 0.05$

Constant ( $\eta = 0.05$ )

$$\omega_0^{(2)} = 2.665, \omega_1^{(2)} = 6.515$$

decaying  $\eta$  [starts with  $\eta = 0.1$ ]

$$\omega_0^{(1)} = 1.665, \omega_1^{(1)} = 0.593$$

$$\omega_0^{(2)} = 2.8424, \omega_1^{(2)} = 7.6101$$

from input table :-

$y = 1 + 2x$  is optimal solution

$$\lambda_1 = 0.069$$

$$\lambda_2 = 0.0449$$

$$H = \begin{bmatrix} 5 & 21 \\ 21 & 121 \end{bmatrix}$$

$$\det(A - \lambda I) = 0$$

$$\therefore \cancel{5} (5 - \lambda) (121 - \lambda) - 21 \times 21 = 0$$

$$\therefore 605 - 5\lambda - 121\lambda + \lambda^2 - 441 = 0$$

$$\therefore \lambda^2 - 126\lambda + 164 = 0$$

$$a = 1, \quad b = -126, \quad c = 164$$

$$\Rightarrow \lambda = \frac{-b \pm \sqrt{b^2 - 4ac}}{2a}$$



$$\therefore \lambda = \frac{-(-126) \pm \sqrt{(126)^2 - 4(1)(164)}}{2 \times 1}$$

$$\lambda = \frac{126 \pm \sqrt{15220}}{2} = 124.6847, 1.3153$$

$$\boxed{\lambda_{\max} = 124.6847}$$

$$\frac{2}{\lambda_{\max}} = 0.016, \text{ for stability}$$

$$\eta < \lambda_{\max},$$

$$\text{i.e., } \eta < 0.016$$

$$\Rightarrow \text{In } (1 \leq \eta \leq 2) \quad \eta = 0.05$$

$$\& \quad \eta_1 = 0.067 \& \eta_2 = 0.049) \neq 0.016$$

$\Rightarrow$  While  $\eta$  improves convergence,  
initial  $\eta$  was aggressive causing

overshooting & instability.

$\therefore$  fast  $c$  decay  $\eta$  didn't improve stability & convergence behaviour compared to constant  $\eta$ .

$\Rightarrow$   $\eta$  in fact made first iteration update larger than constant  $\eta$  therefore overshoot risk.

$\Rightarrow$  Also there is a larger ~~gap~~ gradient leading to instability.

$\Rightarrow$  Both runs produced large jump in parameters



1e) i) from (4)

$$J(w_0, w_1) = 2.5 w_0^2 + 21 w_0 w_1 \\ + 60.5 w_1^2 - 47 w_0 - 263 w_1 \\ + 286.5$$

$$w_0^{(0)} = 2, w_1^{(0)} = 2 \text{ from 2.i) } \nabla J = \begin{bmatrix} 5 \\ 21 \end{bmatrix}$$

$$d = -\nabla J = \begin{bmatrix} -5 \\ -21 \end{bmatrix}$$

$$\phi(\eta) = J(w + \eta d); w_0(\eta) = w_0^{(0)} \\ - \eta \frac{\partial J}{\partial w_0}$$

$$= 2 - \eta(5) = 2 - 5\eta$$

$$\Rightarrow w_1(\eta) = w_1^{(0)} - \eta \frac{\partial J}{\partial w_1} = 2 - \eta(21)$$

$$= 2 - 21\eta$$

## Binary Search

Let current interval be  $[a, b]$

$$\& m = \frac{a+b}{2}$$

$\Rightarrow \phi(m) < \phi(m+\epsilon) \Rightarrow$  fn. is  $\uparrow$  at  $m'$  (slope  $> 0$ )

min. = smaller  $\eta$

$\Rightarrow \phi(m) > \phi(m+\epsilon) \Rightarrow$  fn. is  $\downarrow$  at  $m'$  (slope  $< 0$ )  
min = larger  $\eta$

$\Rightarrow$  Iteration 1 :-

$$[0, 1] \Rightarrow m = \frac{0+1}{2} = 0.5$$

$$\epsilon = 10^{-3} = 0.001$$

$$0.5 + \epsilon = 0.501$$



$$\Rightarrow \phi(0.5) = J(2.5\eta, 2-21\eta)$$

$$= J(2-5(0.5), 2-21(0.5))$$

$$= J(-0.5, -8.5)$$

$$= 2.5(0.5)^2 + 21(-0.5)(-8.5) \\ + 60.5(-8.5)^2 - 47(0.5) \\ - 263(-8.5) + 286.5$$

$$\therefore J(-0.5, -8.5) = \boxed{7006.5}$$

$$\Rightarrow \phi(0.501) = J(2-5 \times 0.501, 2-21 \times 0.501)$$

$$= J(-0.505, -8.521)$$

$$= 2.5(-0.505)^2 + 21(-0.505)(-8.521) \\ + 60.5(-8.521)^2 - 47(-0.505) \\ - 263(-8.521) + 286.5$$

$$\therefore J(-0.505, -8.521) = \boxed{7035.0109}$$

Iteration 2 :-

$$[0, 0.5] \Rightarrow m = \frac{0 + 0.5}{2} = 0.25$$

$$m + \epsilon = 0.25 + 0.001 = 0.251$$

$$\begin{aligned}\phi(0.25) &= J(2 - 5 \times 0.25, 2 - 21 \times 0.25) \\ &= J(0.75, -3.25) \quad \text{--- (9)}\end{aligned}$$

$$\begin{aligned}&= 2.5(0.75)^2 + 21(0.75)(-3.25) \\ &\quad + 60.5(3.25)^2 - 47(0.75) \\ &\quad - 263(-3.25) + 286.5\end{aligned}$$

$$\phi(0.25) = \underline{1695.25} \longrightarrow \text{(9)}$$

$$\begin{aligned}\phi(0.251) &= \phi(0.251) = J(2.5 \times 0.251, \\ &\quad 2 - 21 \times 0.251)\end{aligned}$$

$$\begin{aligned}&= J(0.745, -2.371) \\ &= \boxed{1709.2869}\end{aligned}$$



$\phi(m) < \phi(m+\epsilon)$ , again,

reduced interval =  $[0, 0.25]$

fn is  $\uparrow$  at  $m_2$ , min lies in left.

(ii)  $[a, b] = [0, 1]$ ,  $m_1 = 1/4 = 0.25$ ,

$$m_2 = 3/4 = 0.75$$

$$\phi(0.25) = \int (2 - 5 \times 0.25, 2 - 21 \times 0.25)$$

$$= \int (0.75, -3.25) = \underline{1695.25}$$

$\rightarrow$  From (9)

$$\phi(0.75) = \int (2 - 5 \times 0.75, 2 - 21 \times 0.75)$$

$$= \int (-1.75, -13.75)$$

$$= 2.5 (-1.75)^2 + 21 (-1.75) (-13.75)$$

$$+ 60.5 (-13.75)^2 - 47 (-1.75)$$

$$- 263 (-13.75) + 286.5 = \underline{15936.25}$$

$$\therefore \phi(m_1) < \phi(m_2)$$

$$\therefore \text{min. in } [a, m_2] \text{ i.e.,} \\ [0, 0.75]$$

$$\begin{aligned} \text{(c) (ii) } L &= \text{Interval width} = b - a \\ &= 0.75 - 0 \\ &= 0.75 \end{aligned}$$

$$\Rightarrow \text{golden ratio} \Rightarrow J = \frac{1 + \sqrt{5}}{2} = 0.618$$

$$\begin{aligned} m_1 &= a + (1 - J) \times L = 0 + (1 - 0.618) \\ &\quad \times 0.75 \\ &= \underline{0.2865} \end{aligned}$$

$$\begin{aligned} m_2 &= 0 + J L = 0 + 0.618 \times 0.75 \\ &= \underline{0.4635} \end{aligned}$$



∴ one valid pair

(0.2865, 0.4635) using golden ratio.

→ Another option using specific ratio logic :-

$$m_1 = 0.25 \times 0.75 = 0.1875 \left( \frac{1}{4}^{\text{th}} \text{ of } 1 \text{ way} \right)$$

$$m_2 = 0.75 \times 0.75 = 0.5625$$

$\left( \frac{3}{4}^{\text{th}} \text{ of } 1 \text{ way} \right)$